Commit with normalizer5 (fixpoint, unyieldy) for sound, normalizer with MySN (existential, unwieldy) for completeness, and the beginning of normalizer7 (wouter's SN t -> sig t', normalise t t'), that seems to work!

src/PlutusIR/Semantics/Static/normaliser/STLC_norm_completeness.v
@@ -4,6 +4,144 @@ Import ListNotations.
 
 Require Import Coq.Program.Equality.
 
+Lemma normalise_extend T1 T2 T3 :
+  step_d T1 T2 -> normalise T2 T3 -> normalise T1 T3.
+Proof.
+  intros Hstep Hnorm.
+  generalize dependent T3.
+  induction Hstep; intros T3 Hnorm; try solve [inversion Hnorm; try constructor; eauto].
+  eapply N_BetaReduce; eauto.
+  + apply N_TyLam.
+    admit (* Follows from normalisation__stable'__normal *).
+  + admit.  (* Follows from normalisation__stable'__normal *)
+Admitted.
+
+(* Wouter's suggestion: do not use explicit normalizer in soundness proof*)
+Theorem norm_wouter t :
+  SN5 t -> {t' & normalise t t'}.
+Proof.
+  intros HSN.
+  induction HSN as [t].
+  (* Suppose step_d_f t = None, then t normal, then normalise t t *)
+  assert (Ht_steps: {t' & step_d_f t = Some t'}) by admit.
+  destruct Ht_steps as [t' Ht_steps].
+  specialize (H t' Ht_steps).
+  destruct H as [tn normt'].
+  exists tn.
+  apply normalise_extend with (T2 := t').
+  - now apply step_d_f_to_step_d.
+  - assumption.
+Admitted.
+
+Definition normalizer7' t (snt : SN5 t) :=
+  projT1 (norm_wouter t snt).
+
+Definition normalizer7 t Δ T (Hwt : SN_STLC_named.has_type Δ t T) :=
+  let snt := strong_normalization_d5 Hwt in
+  normalizer7' t snt.
+
+Theorem norm_sound_prrr t tn Δ T (Hwt : SN_STLC_named.has_type Δ t T) :
+  normalizer7 t Δ T Hwt = tn -> normalise t tn.
+Proof.
+  intros.
+  unfold normalizer7 in H.
+  unfold normalizer7' in H.
+  destruct norm_wouter in H.
+  subst.
+  assumption.
+Qed.
+
+Lemma normalise_unique t t' tn1 tn2 :
+  step_d_f t = Some t' -> normalise t tn1 -> normalise t' tn2 -> tn1 = tn2.
+Proof.
+  intros Hstep Hnorm1 Hnorm2.
+
+Admitted.
+
+Lemma norm_lam7 tb x T (snt : (SN5 (tmlam x T tb))) (sntb : SN5 tb):
+  @normalizer7' (tmlam x T tb) snt = tmlam x T (@normalizer7' tb sntb).
+Proof.
+  intros.
+  generalize dependent tb.
+  induction snt as [tlam]; intros sntb.
+  - (* If no step, I think it is easy *)
+    assert (exists tlam', step_d_f tlam = Some tlam') as [tlam' Hstep_tlam] by admit.
+    specialize (H tlam' Hstep_tlam).
+    specialize (H sntb).
+    rewrite <- H.
+    clear.
+    unfold normalizer7'.
+    destruct norm_wouter.
+    destruct norm_wouter.
+    assert (x = x0).
+    {
+      apply (normalise_unique tlam tlam' x x0 Hstep_tlam n n0).
+    }
+    subst.
+    simpl.
+    reflexivity.
+Admitted.
+
+
+(* TODO: DCopied from SubstitutionPreservesTyping/substitueTca
+  In that file it is defined for PlutusIR and proof is started.
+ *)
+Theorem substituteTCA_preserves_kinding : forall T Delta X K U L,
+    SN_STLC_named.has_type ((X, L) :: Delta) T K ->
+    SN_STLC_named.has_type Delta U L ->
+    SN_STLC_named.has_type Delta (substituteTCA X U T) K.
+Admitted.
+
+Theorem norm_complete7 Δ K (t tn : term) (Hwt : SN_STLC_named.has_type Δ t K):
+  normalise t tn -> @normalizer7 t Δ K Hwt = tn.
+Proof.
+  intros HnormR.
+  generalize dependent Δ.
+  generalize dependent K.
+  induction HnormR; intros K' Δ Hwt; subst; auto.
+  - inversion Hwt; subst. (* normalise T1 (tmlam bX K T1n), so T1 is a lambda as well. 
+      What if it is an app before beta reduction?*)
+    (* inversion HnormR1; subst. *)
+    specialize (IHHnormR2 K1 Δ H4).
+    specialize (IHHnormR1 (tp_arrow K1 K') Δ H2). (* we need something like step preserves type? K' = K1 I think*)
+
+    specialize (IHHnormR3 K' Δ). (* The body of the lambda has just type K'*)
+
+    assert (SN_STLC_named.has_type Δ (substituteTCA bX T2n T1n) K').
+    {
+      apply substituteTCA_preserves_kinding with (L := K1).
+      - (* By normalizer preserves typing we have Δ ⊢* (tmlam bX K T1n) : K1 → K'
+              Hence K = K1 and
+              (bX, K1)::Δ ⊢* T1n : K'
+      *) admit.
+      - (* By normalizer preserves typing we have Δ ⊢* T2n : K1  . *)
+        admit.
+    }
+    specialize (IHHnormR3 H).
+    subst.
+    (* eapply norm_subst.
+    exact IHHnormR1. *)
+    admit.
+
+  - 
+    inversion Hwt; subst.
+    rewrite <- (IHHnormR2 K1 Δ H5).
+    specialize (IHHnormR1 (tp_arrow K1 K') Δ H3).
+    subst.
+    admit.
+    (* now apply norm_app. *)
+  - (* Case step_abs *)
+    inversion Hwt; subst.
+    rewrite <- (IHHnormR K2 ((bX, K)::Δ) H4).
+    apply norm_lam7.
+  - unfold normalizer.
+    destruct (strong_normalization_mysn Hwt).
+    unfold normalizer'.
+    (* reflexivity. *)
+Admitted.
+
+
+
 (* Used to do induction over the size of SN proofs *)
 Fixpoint mysn_size {t : term} (HSN : MySN t) : nat :=
   match HSN with
@@ -99,14 +237,6 @@ Proof.
         assumption.
 Qed.
 
-(* TODO: DCopied from SubstitutionPreservesTyping/substitueTca
-  In that file it is defined for PlutusIR and proof is started.
- *)
-Theorem substituteTCA_preserves_kinding : forall T Delta X K U L,
-    SN_STLC_named.has_type ((X, L) :: Delta) T K ->
-    SN_STLC_named.has_type Delta U L ->
-    SN_STLC_named.has_type Delta (substituteTCA X U T) K.
-Admitted.
 
 (* Needs a neutrality requirement *)
 Lemma norm_app t1 t2 (snt : (MySN (tmapp t1 t2))) (snt1 : MySN t1) (snt2 : MySN t2) :
@@ -166,180 +296,40 @@ Proof.
     reflexivity.
 Admitted.
 
-Lemma normalise_extend T1 T2 T3 :
-  step_d T1 T2 -> normalise T2 T3 -> normalise T1 T3.
+Lemma extend_normalizer t1 t2 s (Hstep : step_d_f t1 = Some t2) :
+  @normalizer5' t1 (SNI5 (x := t1) s) =
+  @normalizer5' t2 (s t2 Hstep).
 Proof.
-  intros Hstep Hnorm.
-  generalize dependent T3.
-  induction Hstep; intros T3 Hnorm; try solve [inversion Hnorm; try constructor; eauto].
-  - eapply N_BetaReduce; eauto.
-    + apply N_TyLam.
-      admit (* Follows from normalisation__stable'__normal *).
-    + admit.  
+  induction t1;
+  simpl in Hstep.
 Admitted.
 
-Inductive MySN2 t : Set :=
-| SNI2 : (forall t', step_d_f t = Some t' -> (MySN2 t')) -> MySN2 t. (* TODO: cannot find the inductive step, but removing the existential might work*)
-(* This is the same as the exists, why??? *)
+Theorem norm_sound''' (t tn : term) (snt : SN5 t) :
+  normalise t (normalizer5' snt).
+Proof.
+  induction snt as [t].
+  assert ({t' & step_d_f t = Some t'}) as [t' Hstep] by admit. 
+  specialize (H t' Hstep).
+Admitted.
 
 (* With MySN' t we get the necessary induciton hypothesis! *)
-Theorem norm_sound'' (t tn : term) (snt : MySN t) :
-  normalizer' snt = tn -> normalise t tn.
+Theorem norm_sound'' (t tn : term) (snt : SN5 t) :
+  normalizer5' snt = tn -> normalise t tn.
 Proof.
   intros Hnorm.
-  unfold normalizer in Hnorm.
-  assert (sn2t: MySN2 t) by admit.
-  induction sn2t.
-  (* assume there is a t' s.t. step_d_f t = Some t'*)
-  assert ({t' & step_d_f t = Some t'}) as [t' Hstep] by admit.
-  assert (step_d t t') by admit.
+  induction snt as [t].
+  (* if it does not exist, result is easy by normal is normal, so for no assume it exists*)
+  assert ({t' & step_d_f t = Some t'}) as [t' Hstep] by admit. 
+  assert (step_d t t') by (now apply step_d_f_to_step_d in Hstep).
   apply (normalise_extend t t' tn H0).
-  eapply (H t'); eauto.
   
-    (* should be sn't, but we have to change normalizer' definition first. *)
+  apply (H t') with (e := Hstep).
+  (* We need to show normalizer5' (SN5 t') = tn
+    and we know normalizer5' (SN5 t) = tn ?
+  *)
+  remember ((s t' Hstep) : SN5 t') as snt'.
+  subst.
+  symmetry.
+  exact (extend_normalizer t t' s Hstep).
 Admitted.
 
-Inductive MySN' t : Set :=
-| SNI0' : (step_d_f t = None) -> MySN' t
-| SNI'' : forall t', step_d_f t = Some t' -> (MySN' t') -> MySN' t. (* TODO: cannot find the inductive step, but removing the existential might work*)
-(* This is the same as the exists, why??? *)
-
-(* With MySN' t we get the necessary induciton hypothesis! *)
-Theorem norm_sound' (t tn : term) (snt : MySN t) :
-  normalizer' snt = tn -> normalise t tn.
-Proof.
-  intros Hnorm.
-  unfold normalizer in Hnorm.
-  assert (sn't: MySN' t) by admit.
-  induction sn't.
-  - (* no step: easy *)
-    admit.
-  - assert (step_d t t') by admit.
-    apply (normalise_extend t t' tn H).
-    eapply IHsn't.
-    (* should be sn't*)
-Admitted.
-
-Theorem norm_sound Δ T (t tn : term) (Hwt : SN_STLC_named.has_type Δ t T) :
-    normalizer Hwt = tn -> normalise t tn.
-Proof.
-  intros Hnorm.
-  induction Hnorm.
-  
-  induction Hwt.
-  - unfold normalizer.
-    destruct (strong_normalization_mysn).
-    + simpl.
-      apply N_TyVar.
-    + exfalso.
-      destruct s as [t' [Hstep HSN] ].
-      inversion Hstep.
-  - unfold normalizer.
-    destruct (strong_normalization_mysn).
-    + simpl.
-      apply N_TyLam.
-      unfold normalizer in IHHwt.
-      destruct (strong_normalization_mysn Hwt) in IHHwt.
-      * simpl in IHHwt.
-        assumption.
-      * exfalso.
-        destruct s as [t' [Hstep HSN] ].
-        inversion e.
-        unfold bind in H0.
-        assert (step_d_f T = None).
-        {
-          admit. (* destruct match ???*)
-        } 
-        rewrite Hstep in H.
-        inversion H.
-    + (* lambda steps! *)
-      destruct s as [t' [Hstep HSN] ].
-      unfold normalizer in IHHwt.
-      destruct (strong_normalization_mysn Hwt) in IHHwt.
-      * exfalso.
-        (* lam body no step, while whole lambda steps, contradiction*)
-        admit.
-      * simpl.
-        destruct s as [t'0 [Hstept'0 HSNt'0] ].
-        inversion Hstep.
-        unfold bind in H0.
-        assert (step_d_f T = Some t'0) by admit. (* destruct match *)
-        assert (tmlam X K1 t'0 = t') by admit. (* destruct match *)
-        subst.
-        rewrite norm_lam with (sntb := HSNt'0).
-        apply N_TyLam.
-        simpl in IHHwt.
-        assumption. 
-  - unfold normalizer.
-    remember (SN_STLC_named.K_App Hwt1 Hwt2) as K.
-    remember (mysn_size (strong_normalization_mysn K)) as n.
-    (* generalize dependent Hwt1.
-    generalize dependent K. *)
-    generalize dependent K2.
-    dependent induction n; intros K2 Hwt1 IHHwt1 K HK Hsize.
-    + admit.
-    + destruct (is_neutral (normalizer Hwt1)) eqn:neut.
-      * rewrite norm_app with (snt1 := strong_normalization_mysn Hwt1) (snt2 := strong_normalization_mysn Hwt2).
-        apply N_TyApp.
-        -- simpl in IHHwt1.
-           assumption.
-        -- unfold normalizer in neut.
-          (* is_neutral and neutral_Ty are sound/complete*)
-           admit.
-        -- simpl in IHHwt2.
-           assumption.
-        -- unfold normalizer in neut.
-            admit. (* same case as second..., generate by rewrite norm_app *)
-      * (* not neutral, hence T1n is a lam! Hence we will substitute! *)
-        (* We need to know the shape of T1n, what is the binder name and the kind *)
-
-        assert ({x & {K1 & {T1n & normalizer Hwt1 = tmlam x K1 T1n}}}) as [x [ K1' [ T1n Hnormlam ] ] ] by admit.
-
-        assert (Htypesub: SN_STLC_named.has_type Δ (substituteTCA x (normalizer Hwt2) T1n) K2).
-        {
-          admit.
-        }
-
-        (* rewrite norm_subst with (T1n := T1n) (bX := x) (K1 := K1')
-          (snt1 := strong_normalization_mysn Hwt1) (snt2 := strong_normalization_mysn Hwt2)
-          (snsub := strong_normalization_mysn (Htypesub))
-          . *)
-
-        (*
-
-        We want to use IHn.
-
-        We need n= mysn_size (strong_normalisation_mysn ). We can assume we have it:
-        that T1 = already in normall ambda form and thus T1 = T1n.
-
-        TODO: IHn needs to be generic over kind
-
-
-        Do we have Htypesub = (SN_STLC_named.K_App Hwt1 Hwt2) ? I think so!
-
-        I guess we could use the IH to let tmapp T1 T2 do one step to say T_one.
-        Then this normalises in n steps to (normalizer K).
-
-        Then we know T_one |-> normalizer' (strong_normalization_mysn T_one)
-
-        But also  T_one |-> normalizer' (strong_normalization_mysn (tmapp T1 T2)).
-
-        So we know
-
-        normalise T_one (strong_normalization_mysn (tmapp T1 T2)).
-
-        Then we can use normalise_extend to construct the higher normalise!
-
-        *)
-        specialize (IHn K2 Hwt1 IHHwt1 K HK). (* faulty reasoning, wen eed to do one step or something*)
-        assert (T1 = tmlam x K1' T1n) by admit.
-        subst.
-        eapply N_BetaReduce.
-        -- rewrite Hnormlam in IHHwt1.
-           exact IHHwt1.
-        -- exact IHHwt2.
-        --
-        admit.
-        -- exact Hnormlam.
-
-Admitted.
